crates/algorithms/sha3/proofs/fstar/extraction/Libcrux_sha3.Generic_keccak.Simd128.fst
@@ -183,7 +183,7 @@ let absorb2 (v_RATE: usize) (v_DELIM: u8) (data: t_Array (t_Slice u8) (mk_usize 
 
 #pop-options
 
-#push-options "--fuel 0 --ifuel 1 --z3rlimit 400 --split_queries always --using_facts_from '* -Hacspec_sha3.Sponge.squeeze -EquivImplSpec.Keccakf.Generic.extract_lane'"
+#push-options "--fuel 0 --ifuel 1 --z3rlimit 400 --using_facts_from '* -Hacspec_sha3.Sponge.squeeze -EquivImplSpec.Keccakf.Generic.extract_lane'"
 
 let squeeze2_blocks
       (v_RATE: usize)
